P4 contracts and unified interface for proving contracts

hol/symb_exec/p4_symb_execLib.sig
@@ -6,4 +6,8 @@ val symb_exec:
    hol_type ->
      term -> term -> term list -> term list -> thm -> int -> (thm * thm) list
 
+val p4_symb_exec_prove_contract:
+   hol_type ->
+     term -> term -> term list -> term list -> thm -> int -> term -> thm
+
 end
