hol/symb_exec/p4_symb_exec_test1Script.sml
@@ -149,6 +149,8 @@ val stop_consts_rewr = []
 val stop_consts_never = []
 val path_cond = (ASSUME T)
 val fuel = 2
+val n_max = 50;
+val postcond = “(\s. packet_has_port s 1 \/ packet_has_port s 2):v1model_ascope astate -> bool”;
 (* For debugging:
 val comp_thm = INST_TYPE [Type.alpha |-> arch_ty] arch_multi_exec_comp_n_tl_assl
 *)
@@ -158,89 +160,10 @@ val [(path_cond_res, step_thm), (path_cond2_res, step_thm2)] =
  symb_exec arch_ty ctx init_astate stop_consts_rewr stop_consts_never path_cond 25;
 *)
 
-(* Finishes at 45 steps (one step of which is a symbolic branch)
- * (higher numbers as arguments will work, but do no extra computations) *)
-
-val [(path_cond_res, step_thm), (path_cond2_res, step_thm2)] =
- symb_exec arch_ty ctx init_astate stop_consts_rewr stop_consts_never path_cond 50;
-
 open p4_auxTheory;
 
-(*******************************)
-(* Step 1: prove postcondition *)
-
-(* True if the output packet queue contains a single packet with
- * the provided output port *)
-Definition packet_has_port_def:
- packet_has_port (((i, in_out_list, in_out_list', scope), g_scope_list, arch_frame_list, status):'a astate) port_ok =
-  case in_out_list' of
-    [] => F
-  | [(data, port)] => port = port_ok
-  | _ => F
-End
-
-val postcond = “(\s. packet_has_port s 1 \/ packet_has_port s 2):v1model_ascope astate -> bool”;
-
-Theorem symb_exec_add_postcond:
-!P f s s' Q.
-(P ==> f s = SOME s') ==>
-Q s' ==>
-(P ==> f s = SOME s' /\ Q s')
-Proof
-metis_tac []
-QED
-
-val step_thm' = HO_MATCH_MP symb_exec_add_postcond step_thm;
-val postcond_thm = EQT_ELIM $ SIMP_CONV (srw_ss()) [packet_has_port_def] $ mk_comb (postcond, the_final_state_imp step_thm);
-val step_postcond_thm = MATCH_MP step_thm' postcond_thm;
-
-val step_thm2' = HO_MATCH_MP symb_exec_add_postcond step_thm2;
-val postcond_thm2 = EQT_ELIM $ SIMP_CONV (srw_ss()) [packet_has_port_def] $ mk_comb (postcond, the_final_state_imp step_thm2);
-val step_postcond_thm2 = MATCH_MP step_thm2' postcond_thm2;
-
-(**************************************)
-(* Step 2: rewrite into contract form *)
-
-(* TODO: Eliminate n, put initial state in precondition somehow? *)
-Definition p4_contract_def:
- p4_contract P ctx s n Q =
-  (P ==> arch_multi_exec ctx s n <> NONE /\ !s'. arch_multi_exec ctx s n = SOME s' ==> Q s')
-End
-
-Theorem p4_exec_univ:
-!P ctx s n s' Q.
-(P ==> arch_multi_exec ctx s n = SOME s' /\ Q s') ==>
-p4_contract P ctx s n Q
-(*
-(P ==> arch_multi_exec ctx s n <> NONE /\ !s'. arch_multi_exec ctx s n = SOME s' ==> Q s')
-*)
-Proof
-fs[p4_contract_def]
-QED
-
-val step_postcond_ct_thm = MATCH_MP p4_exec_univ step_postcond_thm
-val step_postcond_ct_thm2 = MATCH_MP p4_exec_univ step_postcond_thm2
-
-(***********************)
-(* Step 3: unification *)
-
-Theorem p4_symb_exec_unify:
-(*
-!P1 P2 f s Q.
-(P1 /\ P2 ==> f s <> NONE /\ !s'. f s = SOME s' ==> Q s') ==>
-(~P1 /\ P2 ==> f s <> NONE /\ !s'. f s = SOME s' ==> Q s') ==>
-P2 ==> f s <> NONE /\ !s'. f s = SOME s' ==> Q s'
-*)
-!P1 P2 ctx s n Q.
-p4_contract (P1 /\ P2) ctx s n Q ==>
-p4_contract (~P1 /\ P2) ctx s n Q ==>
-p4_contract P2 ctx s n Q
-Proof
-fs[p4_contract_def] >>
-metis_tac []
-QED
-
-val thm1 = MATCH_MP p4_symb_exec_unify step_postcond_ct_thm
-val thm2 = MATCH_MP thm1 step_postcond_ct_thm2
+(* Finishes at 45 steps (one step of which is a symbolic branch)
+ * (higher numbers as arguments will work, but do no extra computations) *)
+val contract_thm = p4_symb_exec_prove_contract arch_ty ctx init_astate stop_consts_rewr stop_consts_never path_cond n_max postcond;
 
 val _ = export_theory ();
