hol/symb_exec/p4_symb_execScript.sml
@@ -1,0 +1,43 @@
+open HolKernel boolLib liteLib simpLib Parse bossLib;
+
+open p4Theory;
+
+val _ = new_theory "p4_symb_exec";
+
+Definition packet_has_port_def:
+ packet_has_port (((i, in_out_list, in_out_list', scope), g_scope_list, arch_frame_list, status):'a astate) port_ok =
+  case in_out_list' of
+    [] => F
+  | [(data, port)] => port = port_ok
+  | _ => F
+End
+
+Definition p4_contract_def:
+ p4_contract P ctx s Q =
+  (P ==> ?n. arch_multi_exec ctx s n <> NONE /\ !s'. arch_multi_exec ctx s n = SOME s' ==> Q s')
+End
+
+Theorem p4_symb_exec_to_contract:
+!P ctx s n s' Q.
+(P ==> arch_multi_exec ctx s n = SOME s' /\ Q s') ==>
+p4_contract P ctx s Q
+Proof
+fs[p4_contract_def] >>
+rpt strip_tac >>
+qexists_tac ‘n’ >>
+rpt strip_tac >> (
+ fs[]
+)
+QED
+
+Theorem p4_symb_exec_unify:
+!P1 P2 ctx s Q.
+p4_contract (P1 /\ P2) ctx s Q ==>
+p4_contract (~P1 /\ P2) ctx s Q ==>
+p4_contract P2 ctx s Q
+Proof
+fs[p4_contract_def] >>
+metis_tac []
+QED
+
+val _ = export_theory ();
