hol/symb_exec/symb_execScript.sml
@@ -1,0 +1,14 @@
+open HolKernel boolLib liteLib simpLib Parse bossLib;
+
+val _ = new_theory "symb_exec";
+
+Theorem symb_exec_add_postcond:
+!P f s s' Q.
+(P ==> f s = SOME s') ==>
+Q s' ==>
+(P ==> f s = SOME s' /\ Q s')
+Proof
+metis_tac []
+QED
+
+val _ = export_theory ();
